Launchbury/ArityAnalysisImpl.thy
@@ -26,7 +26,7 @@ lemma thunks_subst_approx:
 nominal_function
   Aexp :: "exp \<Rightarrow> (Arity \<rightarrow> AEnv)"
 where
-  "Aexp (Var x) = (\<Lambda> n . AE_singleton x \<cdot> (up \<cdot> n))"
+  "Aexp (GVar b x) = (\<Lambda> n . AE_singleton x \<cdot> (up \<cdot> n))"
 | "Aexp (Lam [x]. e) = (\<Lambda> n . (Aexp e \<cdot> (pred \<cdot> n)  f|` (fv (Lam [x]. e))))"
 | "Aexp (App e x) = (\<Lambda> n . Aexp e  \<cdot> (inc \<cdot> n) \<squnion> (AE_singleton x \<cdot> (up \<cdot> 0)))"
 | "Aexp (Terms.Let as e) = (\<Lambda> n . (ArityAnalysis.Afix Aexp as \<cdot> (Aexp e \<cdot> n \<squnion> thunks as)) f|` (fv (Terms.Let as e)))"
