Launchbury/Launchbury.thy
@@ -50,7 +50,7 @@ done
 
 lemma eval_test2:
   "y \<noteq> x \<Longrightarrow> n \<noteq> y \<Longrightarrow> n \<noteq> x \<Longrightarrow>[] : (Let [(x, Lam [y]. Var y)] (App (Var x) x)) \<Down>\<^bsub>[]\<^esub> [(x, Lam [y]. Var y)] : (Lam [y]. Var y)"
-  by (auto intro!: Lambda Application Variable Let simp add: fresh_Pair fresh_at_base fresh_Cons fresh_Nil fresh_star_def)
+  by (auto intro!: Lambda Application Variable Let simp add: fresh_Pair fresh_at_base fresh_Cons fresh_Nil fresh_star_def pure_fresh)
 
 subsubsection {* Better introduction rule *}
 
